interleaving/Int0.v
@@ -1,0 +1,48 @@
+Require Import Coqlib.
+(* Require Import ITreelib. *)
+Require Import ImpPrelude.
+(* Require Import STS. *)
+(* Require Import Behavior. *)
+Require Import ModSem.
+Require Import Skeleton.
+(* Require Import PCM. *)
+
+Set Implicit Arguments.
+Set Typeclasses Depth 5.
+
+
+
+
+
+Section PROOF.
+
+  Section BODY.
+    Context {Es: Type -> Type}.
+    Context `{has_pE: pE -< Es}.
+    Context `{has_eventE: eventE -< Es}.
+    Definition spwanF: (list val) -> itree Es val :=
+      fun varg =>
+        z <- trigger (Syscall "spawn" varg↑ top1);; Ret Vundef.
+              
+    Definition yieldF: (list val) -> itree Es val :=
+      fun varg =>
+        z <- trigger (Syscall "yield" varg↑ top1);; Ret Vundef.
+
+  End BODY.
+
+
+
+  Definition IntSem (sk: Sk.t): ModSem.t :=
+    {|
+      ModSem.fnsems := [("spwan", cfunU spwanF) ; ("yield", cfunU yieldF)];
+      ModSem.mn := "Int";
+      ModSem.initial_st := Vundef↑;
+    |}
+  .
+
+  Definition Mem: Mod.t := {|
+    Mod.get_modsem := IntSem;
+    Mod.sk := Sk.unit;
+  |}
+  .
+End PROOF.
